theories/SepFunctor.v
@@ -268,8 +268,6 @@ Implicit Types P : Prop.
 
 Notation "'\exists' x1 , H" := (hexists (fun x1 => H))
   (at level 39, x1 ident, H at level 50) : heap_scope.
-Notation "'\exists' x1 x2 , H" := (\exists x1, \exists x2, H)
-  (at level 39, x1 ident, x2 ident, H at level 50) : heap_scope.
 Notation "'\exists' x1 x2 x3 , H" := (\exists x1, \exists x2, \exists x3, H)
   (at level 39, x1 ident, x2 ident, x3 ident, H at level 50) : heap_scope.
 Notation "'\exists' x1 x2 x3 x4 , H" :=
@@ -279,12 +277,18 @@ Notation "'\exists' x1 x2 x3 x4 x5 , H" :=
   (\exists x1, \exists x2, \exists x3, \exists x4, \exists x5, H)
   (at level 39, x1 ident, x2 ident, x3 ident, x4 ident, x5 ident, H at level 50) : heap_scope.
 
+(* TODO: get this definition to work:
+Notation "'\exists' x1 .. xn , H" := 
+  (hexists (fun x1 => .. (hexists (fun xn => H)) ..))
+  (at level 39, x1, xn ident, H at level 50) : heap_scope.
+*)
+
 Notation "'\exists' ( x1 : T1 ) , H" := (hexists (fun x1:T1 => H))
   (at level 39, x1 ident, H at level 50, only parsing) : heap_scope.
 Notation "'\exists' ( x1 : T1 ) ( x2 : T2 ) , H" := (\exists (x1:T1), \exists (x2:T2), H)
-  (at level 39, x1 ident, x2 ident, H at level 50) : heap_scope.
+  (at level 39, x1 ident, x2 ident, H at level 50, only parsing) : heap_scope.
 Notation "'\exists' ( x1 : T1 ) ( x2 : T2 ) ( x3 : T3 ) , H" := (\exists (x1:T1), \exists (x2:T2), \exists (x3:T3), H)
-  (at level 39, x1 ident, x2 ident, x3 ident, H at level 50) : heap_scope.
+  (at level 39, x1 ident, x2 ident, x3 ident, H at level 50, only parsing) : heap_scope.
 
 (** Notation for [hforall] *)
 
